source/docs/bv_expriments/garbage.dfy
@@ -1,50 +1,103 @@
 // related to mark and sweep
-datatype Color = White | Gray | Black | Bad
+// datatype Color = White | Gray | Black | Bad
 
-function interpret(bucket: bv32, index: int) : seq<Color> 
-    requires 0<=index<=15
-    decreases(16-index);  
+// function interpret(bucket: bv32, index: int) : seq<Color> 
+//     requires 0<=index<=15
+//     decreases(16-index);  
+// {
+//     var mask:bv32 := 3;
+//     var bucket := bucket >> (index*2);
+//     var color_bit: bv32 := bucket & mask;
+//     var c : Color := 
+//     if color_bit == 0 then
+//         White
+//     else if color_bit == 1 then
+//         Gray
+//     else if color_bit == 2 then
+//         Black
+//     else
+//         Bad;
+
+//     if index== 15 then 
+//         [c]
+//     else 
+//         interpret(bucket, index+1) + [c]
+// }
+
+// method set_color(bucket: bv32, c:Color, index: int, ghost g_bucket: seq<Color>) returns (new_bucket:bv32) 
+//   requires 0<= index < 16;
+//   requires interpret(bucket, 0) == g_bucket;
+//   ensures interpret(new_bucket, 0) == g_bucket[index := c];
+// {
+//     var mask:bv32 := 3;
+//     mask := mask << (index*2);
+//     mask := !mask;
+//     new_bucket := bucket & mask;
+
+//     var num_color:bv32 := 
+//         if c == White then
+//             0
+//         else if c == Gray then
+//             1
+//         else if c == Black then
+//             2
+//         else
+//             3;
+    
+//     num_color := num_color << (index*2);
+//     new_bucket := new_bucket | num_color;
+// }
+
+type uint5  = i :int | 0 <= i < 32
+type uint32 = i :int | 0 <= i < 4294967296
+
+function method get_bit(bv: uint32, i: uint5): bool
+
+function method set_bit(bv: uint32, i: uint5, b: bool): (bv': uint32)
+    ensures forall j: uint5 :: (j != i) ==> (get_bit(bv', j) == get_bit(bv, i))
+    ensures get_bit(bv', i) == b
+
+function I_aux(bv: uint32, i: uint5): seq<bool>
 {
-    var mask:bv32 := 3;
-    var bucket := bucket >> (index*2);
-    var color_bit: bv32 := bucket & mask;
-    var c : Color := 
-    if color_bit == 0 then
-        White
-    else if color_bit == 1 then
-        Gray
-    else if color_bit == 2 then
-        Black
+    if i == 0 then
+        [get_bit(bv, 0)]
     else
-        Bad;
-
-    if index== 15 then 
-        [c]
-    else 
-        interpret(bucket, index+1) + [c]
+       I_aux(bv, i - 1) + [get_bit(bv, i)]
 }
 
-method set_color(bucket: bv32, c:Color, index: int, ghost g_bucket: seq<Color>) returns (new_bucket:bv32) 
-  requires 0<= index < 16;
-  requires interpret(bucket, 0) == g_bucket;
-  ensures interpret(new_bucket, 0) == g_bucket[index := c];
+lemma I_aux_correspond(bv: uint32, i: uint5)
+    ensures |I_aux(bv, i)| == i + 1
+    ensures forall j: uint5 :: (j < i) ==> I_aux(bv, i)[j] == get_bit(bv, j)
 {
-    var mask:bv32 := 3;
-    mask := mask << (index*2);
-    mask := !mask;
-    new_bucket := bucket & mask;
+    if i != 0 {
+        I_aux_correspond(bv, i - 1);
+        var preI := I_aux(bv, i - 1);
+        var curI := I_aux(bv, i);
 
-    var num_color:bv32 := 
-        if c == White then
-            0
-        else if c == Gray then
-            1
-        else if c == Black then
-            2
-        else
-            3;
-    
-    num_color := num_color << (index*2);
-    new_bucket := new_bucket | num_color;
+        assert forall j: uint5 :: (j < i - 1) ==> preI[j] == get_bit(bv, j);
+        assert preI + [get_bit(bv, i)] == curI;
+
+        forall j: uint5
+            ensures j < i ==> curI[j] == get_bit(bv, j);
+        {
+            if j < i - 1 {
+                assert curI[j] == preI[j];
+            } else if j < i {
+                assert j == i - 1;
+                assert curI[j] == get_bit(bv, j);
+            }
+        }
+    }
 }
-    
+
+function I(bv: uint32): seq<bool>
+{
+    I_aux(bv, 31)
+}
+
+lemma I_correspond(bv: uint32)
+    ensures |I(bv)| == 32
+    ensures forall i: uint5 :: I(bv)[i] == get_bit(bv, i)
+{
+    I_aux_correspond(bv, 31);
+}
